zoo_partition: Replace set of descriptors by map.

theories/zoo_partition/partition.v
@@ -30,14 +30,16 @@ Implicit Types part : gset (gset location).
 Implicit Types γ : gname.
 
 Record partition_descr := {
-  partition_descr_class : location ;
   partition_descr_elts : list location ;
+  partition_descr_prev : location ;
+  partition_descr_next : location ;
 }.
 
 #[local] Instance partition_descr_inhabited : Inhabited partition_descr :=
   populate {|
-    partition_descr_class := inhabitant ;
     partition_descr_elts := inhabitant ;
+    partition_descr_prev := inhabitant ;
+    partition_descr_next := inhabitant ;
   |}.
 #[local] Instance partition_descr_eq_dec : EqDecision partition_descr :=
   ltac:(solve_decision).
@@ -48,7 +50,7 @@ Proof.
 Qed.
 
 Implicit Types descr : partition_descr.
-Implicit Types descrs : gset partition_descr.
+Implicit Types descrs : gmap location partition_descr.
 
 Class PartitionG Σ `{zoo_G : !ZooG Σ} := {
   #[local] partition_G_elts_G :: MonoSetG Σ location ;
@@ -72,31 +74,31 @@ Section partition_G.
   #[local] Definition partition_elts_elem γ elt :=
     mono_set_elem γ elt.
 
-  #[local] Definition partition_model_elt descr elt : iProp Σ :=
-    elt.[class_] ↦ #descr.(partition_descr_class) ∗
+  #[local] Definition partition_model_elt class descr elt : iProp Σ :=
+    elt.[class_] ↦ #class ∗
     elt.[seen] ↦ #false.
   #[local] Instance : CustomIpatFormat "model_elt" :=
     "(
       Helt{}_class{_{suff}} &
       Helt{}_seen{_{suff}}
     )".
-  #[local] Definition partition_model_descr descrs descr : iProp Σ :=
+  #[local] Definition partition_descr_model class descrs descr : iProp Σ :=
     ∃ first last prev_descr prev next_descr next,
     ⌜head descr.(partition_descr_elts) = Some first⌝ ∗
     ⌜list.last descr.(partition_descr_elts) = Some last⌝ ∗
-    ⌜prev_descr ∈ descrs⌝ ∗
+    ⌜descrs !! descr.(partition_descr_prev) = Some prev_descr⌝ ∗
     ⌜list.last prev_descr.(partition_descr_elts) = Some prev⌝ ∗
-    ⌜next_descr ∈ descrs⌝ ∗
+    ⌜descrs !! descr.(partition_descr_next) = Some next_descr⌝ ∗
     ⌜head next_descr.(partition_descr_elts) = Some next⌝ ∗
-    descr.(partition_descr_class).[first] ↦ #first ∗
-    descr.(partition_descr_class).[last] ↦ #last ∗
-    descr.(partition_descr_class).[len] ↦ #(length descr.(partition_descr_elts)) ∗
-    descr.(partition_descr_class).[split] ↦ #first ∗
-    descr.(partition_descr_class).[split_len] ↦ #0 ∗
+    class.[first] ↦ #first ∗
+    class.[last] ↦ #last ∗
+    class.[len] ↦ #(length descr.(partition_descr_elts)) ∗
+    class.[split] ↦ #first ∗
+    class.[split_len] ↦ #0 ∗
     xdlchain #prev descr.(partition_descr_elts) #next ∗
     [∗ list] elt ∈ descr.(partition_descr_elts),
-      partition_model_elt descr elt.
-  #[local] Instance : CustomIpatFormat "model_descr" :=
+      partition_model_elt class descr elt.
+  #[local] Instance : CustomIpatFormat "descr_model" :=
     "(
       %first{} &
       %last{} &
@@ -119,19 +121,19 @@ Section partition_G.
       Helts{}
     )".
   #[local] Definition partition_model' γ descrs : iProp Σ :=
-    partition_elts_auth γ ([∪ set] descr ∈ descrs, list_to_set descr.(partition_descr_elts)) ∗
-    [∗ set] descr ∈ descrs,
-      partition_model_descr descrs descr.
-  #[local] Instance : CustomIpat0 "model'" :=
+    partition_elts_auth γ ([∪ map] descr ∈ descrs, list_to_set descr.(partition_descr_elts)) ∗
+    [∗ map] class ↦ descr ∈ descrs,
+      partition_descr_model class descrs descr.
+  #[local] Instance : CustomIpatFormat "model'" :=
     "(
       Helts_auth &
       Hdescrs
     )".
   Definition partition_model γ part : iProp Σ :=
     ∃ descrs,
-    ⌜part = set_map (list_to_set ∘ partition_descr_elts) descrs⌝ ∗
+    ⌜part = map_to_set (λ _, list_to_set ∘ partition_descr_elts) descrs⌝ ∗
     partition_model' γ descrs.
-  #[local] Instance : CustomIpat0 "model" :=
+  #[local] Instance : CustomIpatFormat "model" :=
     "(
       %descrs &
       -> &
@@ -185,92 +187,63 @@ Section partition_G.
     apply mono_set_insert'.
   Qed.
 
-  #[local] Lemma partition_model_disjoint_strong {γ descrs} descr1 descr2 :
-    descr1 ∈ descrs →
-    descr2 ∈ descrs →
-    partition_model' γ descrs ⊢
-      ⌜ descr1 ≠ descr2 →
-        descr1.(partition_descr_class) ≠ descr2.(partition_descr_class)
-      ⌝ ∗
-      ⌜ ∀ elt,
-        elt ∈ descr1.(partition_descr_elts) →
-        elt ∈ descr2.(partition_descr_elts) →
-        descr1 = descr2
-      ⌝.
-  Proof.
-    iIntros "%Hdescrs_elem_1 %Hdescrs_elem_2 (:model')".
-    destruct (decide (descr1 = descr2)) as [<- | Hneq]; first done.
-    iDestruct (big_sepS_delete _ _ descr1 with "Hdescrs") as "((:model_descr =1) & Hdescrs)"; first done.
-    iDestruct (big_sepS_elem_of _ _ descr2 with "Hdescrs") as "(:model_descr =2)"; first set_solver.
-    iSplit.
-    - iIntros "_ <-".
-      iApply (pointsto_exclusive with "Hclass1_first Hclass2_first").
-    - iIntros (elt (i1 & Hlookup_1)%elem_of_list_lookup (i2 & Hlookup_2)%elem_of_list_lookup).
-      iDestruct (big_sepL_lookup with "Helts1") as "(:model_elt suff=1)"; first done.
-      iDestruct (big_sepL_lookup with "Helts2") as "(:model_elt suff=2)"; first done.
-      iDestruct (pointsto_exclusive with "Helt_class_1 Helt_class_2") as %[].
-  Qed.
-  #[local] Lemma partition_model_class_unique {γ descrs} descr1 descr2 :
-    descr1 ∈ descrs →
-    descr2 ∈ descrs →
-    descr1 ≠ descr2 →
-    partition_model' γ descrs ⊢
-    ⌜descr1.(partition_descr_class) ≠ descr2.(partition_descr_class)⌝.
-  Proof.
-    iIntros "%Hdescrs_elem_1 %Hdescrs_elem_2 %Hneq Hmodel".
-    iDestruct (partition_model_disjoint_strong descr1 descr2 with "Hmodel") as "(% & _)"; [done.. |].
-    iSteps.
-  Qed.
-  #[local] Lemma partition_model_disjoint' {γ descrs} elt descr1 descr2 :
-    descr1 ∈ descrs →
+  #[local] Lemma partition_model_disjoint' {γ descrs} class1 descr1 class2 descr2 elt :
+    descrs !! class1 = Some descr1 →
     elt ∈ descr1.(partition_descr_elts) →
-    descr2 ∈ descrs →
+    descrs !! class2 = Some descr2 →
     elt ∈ descr2.(partition_descr_elts) →
     partition_model' γ descrs ⊢
-    ⌜descr1 = descr2⌝.
+      ⌜class1 = class2⌝ ∗
+      ⌜descr1 = descr2⌝.
   Proof.
-    iIntros "%Hdescrs_elem_1 %Hdescr1_elem %Hdescrs_elem_2 %Hdescr2_elem Hmodel".
-    iDestruct (partition_model_disjoint_strong descr1 descr2 with "Hmodel") as "(_ & %)"; [done.. |].
-    iSteps.
+    iIntros (Hdescrs_lookup_1 (i1 & Helts1_lookup)%elem_of_list_lookup Hdescrs_lookup_2 (i2 & Helts2_lookup)%elem_of_list_lookup) "(:model')".
+    destruct (decide (class1 = class2)) as [<- | Hneq]; first naive_solver.
+    iDestruct (big_sepM_delete _ _ class1 with "Hdescrs") as "((:descr_model =1) & Hdescrs)"; first done.
+    iDestruct (big_sepM_lookup _ _ class2 with "Hdescrs") as "(:descr_model =2)".
+    { rewrite lookup_delete_ne //. }
+    iDestruct (big_sepL_lookup with "Helts1") as "(:model_elt suff=1)"; first done.
+    iDestruct (big_sepL_lookup with "Helts2") as "(:model_elt suff=2)"; first done.
+    iDestruct (pointsto_exclusive with "Helt_class_1 Helt_class_2") as %[].
   Qed.
-  #[local] Lemma partition_model_disjoint'' {γ descrs} elt descr :
-    descr ∈ descrs →
+  #[local] Lemma partition_model_disjoint'' {γ descrs} class descr elt :
+    descrs !! class = Some descr →
     elt ∈ descr.(partition_descr_elts) →
     partition_model' γ descrs ⊢
-    ⌜ ∀ descr',
-      descr' ∈ descrs →
+    ⌜ ∀ class' descr',
+      descrs !! class' = Some descr' →
       elt ∈ descr'.(partition_descr_elts) →
-      descr' = descr
+        class' = class ∧
+        descr' = descr
     ⌝.
   Proof.
-    iIntros "%Hdescrs_elem %Helt_elem Hmodel %descr' %Hdescr_elem' %Helts_elem'".
-    iApply (partition_model_disjoint' with "Hmodel"); done.
+    iIntros "%Hdescrs_lookup %Helts_elem Hmodel %class' %descr' %Hdescrs_lookup' %Helts_elem'".
+    iDestruct (partition_model_disjoint' class _ class' with "Hmodel") as %(<- & <-); done.
   Qed.
   #[local] Lemma partition_elt_valid' γ descrs elt v :
     partition_model' γ descrs -∗
     partition_elt γ elt v -∗
-      ∃ descr,
-      ⌜descr ∈ descrs⌝ ∗
-      ⌜elt ∈ descr.(partition_descr_elts)⌝ ∧
-      ⌜ ∀ descr',
-        descr' ∈ descrs →
+      ∃ class descr,
+      ⌜descrs !! class = Some descr⌝ ∗
+      ⌜elt ∈ descr.(partition_descr_elts)⌝ ∗
+      ⌜ ∀ class' descr',
+        descrs !! class' = Some descr' →
         elt ∈ descr'.(partition_descr_elts) →
-        descr' = descr
+          class' = class ∧
+          descr' = descr
       ⌝.
   Proof.
     iIntros "(:model') (:elt)".
-    iDestruct (partition_elts_elem_valid with "Helts_auth Helts_elem") as %(descr & Hdescr & Helts_elem%elem_of_list_to_set)%big_unionS_elem_of.
-    iExists descr. iStep 5 as (descr' Hdescr' Helts_elem').
-    iApply partition_model_disjoint'; [done.. |].
-    iSteps.
+    iDestruct (partition_elts_elem_valid with "Helts_auth Helts_elem") as %(class & descr & Hdescrs_lookup & Helts_elem%elem_of_list_to_set)%big_unionM_elem_of.
+    iStep 2.
+    iApply (partition_model_disjoint'' with "[$]"); done.
   Qed.
-  #[local] Lemma partition_model_descr_elts_NoDup {γ descrs} descr :
-    descr ∈ descrs →
+  #[local] Lemma partition_descr_model_elts_NoDup {γ descrs} class descr :
+    descrs !! class = Some descr →
     partition_model' γ descrs ⊢
     ⌜NoDup descr.(partition_descr_elts)⌝.
   Proof.
     iIntros "%Hdescrs_lookup (:model')".
-    iDestruct (big_sepS_elem_of with "Hdescrs") as "(:model_descr)"; first done.
+    iDestruct (big_sepM_lookup with "Hdescrs") as "(:descr_model)"; first done.
     iApply (xdlchain_NoDup with "Hchain").
   Qed.
 
@@ -280,9 +253,7 @@ Section partition_G.
       partition_model γ ∅.
   Proof.
     iMod partition_elts_alloc as "(%γ & Helts_auth)".
-    iExists γ, ∅.
-    rewrite set_map_empty /partition_model' !big_opS_empty.
-    iSteps.
+    iExists γ, ∅. rewrite /partition_model' !big_opM_empty. iSteps.
   Qed.
   Lemma partition_model_non_empty {γ part} cl :
     cl ∈ part →
@@ -291,8 +262,8 @@ Section partition_G.
   Proof.
     iIntros "%Hcl (:model)".
     iDestruct "Hmodel" as "(:model')".
-    apply elem_of_map in Hcl as (descr & -> & Hdescr).
-    iDestruct (big_sepS_elem_of with "Hdescrs") as "(:model_descr)"; first done.
+    apply elem_of_map_to_set in Hcl as (class & descr & Hdescrs_lookup & <-).
+    iDestruct (big_sepM_lookup with "Hdescrs") as "(:descr_model)"; first done.
     iPureIntro. eapply list_to_set_not_empty, hd_error_some_nil. done.
   Qed.
   Lemma partition_model_disjoint {γ part} elt cl1 cl2 :
@@ -303,14 +274,12 @@ Section partition_G.
     partition_model γ part ⊢
     ⌜cl1 = cl2⌝.
   Proof.
-    iIntros "%Hpart_elem_1 %Hcl1_elem %Hpart_elem_2 %Hcl2_elem (:model)".
-    apply elem_of_map in Hpart_elem_1 as (descr1 & -> & Hdescrs_elem_1).
-    apply elem_of_map in Hpart_elem_2 as (descr2 & -> & Hdescrs_elem_2).
-    iDestruct (partition_model_disjoint' elt descr1 descr2 with "Hmodel") as %<-; last iSteps.
-    { done. }
-    { apply elem_of_list_to_set in Hcl1_elem. done. }
-    { done. }
-    { apply elem_of_list_to_set in Hcl2_elem. done. }
+    iIntros (Hpart_elem_1 Hcl1_elem Hpart_elem_2 Hcl2_elem) "(:model)".
+    apply elem_of_map_to_set in Hpart_elem_1 as (class1 & descr1 & Hdescrs_lookup_1 & <-).
+    apply elem_of_list_to_set in Hcl1_elem.
+    apply elem_of_map_to_set in Hpart_elem_2 as (class2 & descr2 & Hdescrs_lookup_2 & <-).
+    apply elem_of_list_to_set in Hcl2_elem.
+    iDestruct (partition_model_disjoint' class1 descr1 class2 descr2 with "Hmodel") as %(<- & <-); done.
   Qed.
 
   Lemma partition_elt_valid γ part elt v :
@@ -321,9 +290,9 @@ Section partition_G.
       ⌜elt ∈ cl⌝.
   Proof.
     iIntros "(:model) Helt".
-    iDestruct (partition_elt_valid' with "Hmodel Helt") as "(%descr & %descrs_elem & %Helts_elem & _)".
+    iDestruct (partition_elt_valid' with "Hmodel Helt") as "(%class & %descr & %Hdescrs_lookup & %Helts_elem & _)".
     iExists (list_to_set descr.(partition_descr_elts)). iSplit; iPureIntro.
-    - apply elem_of_map. naive_solver.
+    - apply elem_of_map_to_set. naive_solver.
     - rewrite elem_of_list_to_set //.
   Qed.
   Lemma partition_elt_agree γ elt v1 v2 :
@@ -358,30 +327,30 @@ Section partition_G.
       partition_elt γ elt v
     }}}
       (#elt).{class_}
-    {{{ descr,
-      RET #descr.(partition_descr_class);
+    {{{ class descr,
+      RET #class;
       partition_model' γ descrs ∗
       partition_elt γ elt v ∗
-      ⌜descr ∈ descrs⌝ ∗
+      ⌜descrs !! class = Some descr⌝ ∗
       ⌜elt ∈ descr.(partition_descr_elts)⌝ ∗
-      ⌜ ∀ descr',
-        descr' ∈ descrs →
+      ⌜ ∀ class' descr',
+        descrs !! class' = Some descr' →
         elt ∈ descr'.(partition_descr_elts) →
-        descr' = descr
+          class' = class ∧
+          descr' = descr
       ⌝
     }}}.
   Proof.
     iIntros "%Φ (Hmodel & Helt) HΦ".
-    iDestruct (partition_elt_valid' with "Hmodel Helt") as "(%descr & %Hdescrs_elem & %Helts_elem & %Hdescr)".
+    iDestruct (partition_elt_valid' with "Hmodel Helt") as "(%class & %descr & %Hdescrs_lookup & %Helts_elem & %Helt)".
     iDestruct "Hmodel" as "(:model')".
-    iDestruct (big_sepS_elem_of_acc with "Hdescrs") as "((:model_descr) & Hdescrs)"; first done.
+    iDestruct (big_sepM_lookup_acc with "Hdescrs") as "((:descr_model) & Hdescrs)"; first done.
     odestruct elem_of_list_lookup_1 as (i & Helts_lookup); first done.
     iDestruct (big_sepL_lookup_acc with "Helts") as "((:model_elt) & Helts)"; first done.
     wp_load.
     iDestruct ("Helts" with "[$]") as "Helts".
-    iDestruct ("Hdescrs" with "[- Helts_auth Helt HΦ]") as "Hdescrs".
-    { iExists first, last, prev_descr, prev, next_descr, next. iSteps. }
-    iSteps.
+    iDestruct ("Hdescrs" with "[- Helts_auth Helt HΦ]") as "Hdescrs"; first iSteps.
+    iSteps; naive_solver.
   Qed.
 
   Lemma partition_make_spec γ part v :
@@ -403,34 +372,35 @@ Section partition_G.
     wp_block class as "(Hclass_first & Hclass_last & Hclass_len & Hclass_split & Hclass_split_len & _)".
     wp_store. wp_pures.
 
-    pose descr := {|
-      partition_descr_class := class ;
-      partition_descr_elts := [elt] ;
-    |}.
-    iMod (partition_elts_insert elt with "Helts_auth") as "(Helts_auth & #Helts_elem)".
-
-    iAssert ⌜descr ∉ descrs⌝%I as %Hdescr.
-    { iIntros "%Hdescrs_elem".
-      iDestruct (big_sepS_elem_of with "Hdescrs") as "(:model_descr =')"; first done.
+    iAssert ⌜descrs !! class = None⌝%I as %Hclass.
+    { rewrite -eq_None_ne_Some. iIntros "%descr %Hdescrs_lookup".
+      iDestruct (big_sepM_lookup with "Hdescrs") as "(:descr_model =')"; first done.
       iApply (pointsto_exclusive with "Hclass_first Hclass'_first").
     }
 
-    iApply "HΦ". iModIntro.
-    iSplitL; last iSteps.
-    iExists ({[descr]} ∪ descrs).
-    iSplit.
-    { iPureIntro. rewrite set_map_union_L set_map_singleton_L /= right_id_L (comm_L (∪)) //. }
+    pose descr := {|
+      partition_descr_elts := [elt] ;
+      partition_descr_prev := class ;
+      partition_descr_next := class ;
+    |}.
+    iMod (partition_elts_insert elt with "Helts_auth") as "(Helts_auth & #Helts_elem)".
+
+    iApply "HΦ".
+    iModIntro. iSplitL; last iSteps.
+    iExists (<[class := descr]> descrs). iSplit.
+    { iPureIntro.
+      rewrite map_to_set_insert_L //= right_id_L. set_solver.
+    }
     iSplitL "Helts_auth".
     { iApply (mono_set_auth_proper with "Helts_auth").
-      rewrite big_opS_insert //. set_solver.
+      rewrite big_opM_insert //. set_solver.
     }
-    iApply (big_sepS_insert_2 with "[- Hdescrs] [Hdescrs]").
+    iApply (big_sepM_insert_2 with "[- Hdescrs] [Hdescrs]").
     - iExists elt, elt, descr, elt, descr, elt.
-      rewrite xdlchain_singleton.
-      iSteps; iPureIntro; set_solver.
-    - iApply (big_sepS_impl with "Hdescrs"). iIntros "!> %descr' %Hdescrs_elem (:model_descr)".
+      rewrite xdlchain_singleton lookup_insert //. iSteps.
+    - iApply (big_sepM_impl with "Hdescrs"). iIntros "!> %class' %descr' %Hdescrs_lookup' (:descr_model)".
       iExists first, last, prev_descr, prev, next_descr, next.
-      iSteps; iPureIntro; set_solver.
+      rewrite !lookup_insert_ne //; [naive_solver.. |]. iSteps.
   Qed.
 
   Lemma partition_make_same_class_spec γ part elt v v' :
@@ -454,7 +424,7 @@ Section partition_G.
     iIntros "%Φ ((:model) & Helt) HΦ".
 
     wp_rec.
-    wp_smart_apply (partition_get_class_spec with "[$Hmodel $Helt]") as (descr) "(Hmodel & Helt & %Hdescrs_elem & %Helts_elem & %Helt_descr)".
+    wp_smart_apply (partition_get_class_spec with "[$Hmodel $Helt]") as (class descr) "(Hmodel & Helt & %Hdescrs_lookup & %Helts_elem & %Helt)".
     wp_smart_apply (partition_dllist_create_spec with "[//]") as (elt') "(Helt'_prev & Helt'_next & #Helt'_data & Helt'_class & Helt'_seen)".
   Admitted.
 
@@ -507,22 +477,19 @@ Section partition_G.
   Proof.
     iIntros "%Φ ((:model) & Helt1 & Helt2) HΦ".
     wp_rec.
-    wp_smart_apply (partition_get_class_spec with "[$Hmodel $Helt2]") as (descr2) "(Hmodel & Helt2 & %Hdescrs_elem_2 & %Helts_elem_2 & %Hdescr2)".
-    wp_apply (partition_get_class_spec with "[$Hmodel $Helt1]") as (descr1) "(Hmodel & Helt1 & %Hdescrs_elem_1 & %Helts_elem_1 & %Hdescr1)".
-    wp_pures.
-    destruct (decide (descr1 = descr2)) as [<- | Hneq].
-    - rewrite bool_decide_eq_true_2 //.
-      iSteps as (cl1 cl2 (descr1' & -> & Hdescrs_elem_1')%elem_of_map Hcl1_elem (descr2' & -> & Hdescrs_elem_2')%elem_of_map Hcl2_elem) / --silent. iPureIntro.
-      rewrite !elem_of_list_to_set in Hcl1_elem Hcl2_elem.
-      opose proof* Hdescr1 as ->; [done.. |].
-      opose proof* Hdescr2 as <-; [done.. |].
-      done.
-    - iDestruct (partition_model_class_unique descr1 descr2 with "Hmodel") as %?; [done.. |].
-      rewrite bool_decide_eq_false_2 //.
-      iSteps as (cl Hcl_elem_1 (descr & -> & Hdescrs_elem)%elem_of_map _ Hcl_elem_2) / --silent. iPureIntro.
-      rewrite !elem_of_list_to_set in Hcl_elem_1 Hcl_elem_2.
-      opose proof* Hdescr1 as Heq1; [done.. |].
-      opose proof* Hdescr2 as Heq2; [done.. |].
+    wp_smart_apply (partition_get_class_spec with "[$Hmodel $Helt2]") as (class2 descr2) "(Hmodel & Helt2 & %Hdescrs_lookup_2 & %Helts2_elem & %Helt2)".
+    wp_apply (partition_get_class_spec with "[$Hmodel $Helt1]") as (class1 descr1) "(Hmodel & Helt1 & %Hdescrs_lookup_1 & %Helts1_elem & %Helt1)".
+    wp_pures. case_bool_decide as Hcase.
+    - subst class2.
+      iSteps as (cl1 cl2 (class1' & descr1' & Hdescrs_lookup_1' & <-)%elem_of_map_to_set Helts1'_elem (class2' & descr2' & Hdescrs_lookup_2' & <-)%elem_of_map_to_set Helts2'_elem) / --silent. iPureIntro.
+      rewrite !elem_of_list_to_set in Helts1'_elem Helts2'_elem.
+      edestruct (Helt1 class1' descr1') as (-> & ->); [done.. |].
+      edestruct (Helt2 class2' descr2') as (-> & ->); [done.. |].
+      congruence.
+    - iSteps as (cl Helts_elem_1 (class & descr & Hdescrs_lookup & <-)%elem_of_map_to_set _ Helts_elem_2) / --silent. iPureIntro.
+      rewrite !elem_of_list_to_set in Helts_elem_1 Helts_elem_2.
+      edestruct (Helt1 class descr) as (<- & <-); [done.. |].
+      edestruct (Helt2 class descr) as (<- & <-); [done.. |].
       congruence.
   Qed.
 
@@ -544,15 +511,14 @@ Section partition_G.
   Proof.
     iIntros "%Φ ((:model) & Helt) HΦ".
     wp_rec.
-    wp_apply (partition_get_class_spec with "[$Hmodel $Helt]") as (descr) "(Hmodel & Helt & %Hdescrs_elem & %Helts_elem & %Helt_descr)".
+    wp_apply (partition_get_class_spec with "[$Hmodel $Helt]") as (class descr) "(Hmodel & Helt & %Hdescrs_lookup & %Helts_elem & %Helt)".
     iDestruct "Hmodel" as "(:model')".
-    iDestruct (big_sepS_elem_of_acc with "Hdescrs") as "((:model_descr) & Hdescrs)"; first done.
+    iDestruct (big_sepM_lookup_acc with "Hdescrs") as "((:descr_model) & Hdescrs)"; first done.
     wp_load.
-    iDestruct ("Hdescrs" with "[- Helts_auth Helt HΦ]") as "Hdescrs".
-    { iExists first, last, prev_descr, prev, next_descr, next. iSteps. }
+    iDestruct ("Hdescrs" with "[- Helts_auth Helt HΦ]") as "Hdescrs"; first iSteps.
     apply head_Some_elem_of in Hfirst.
-    iDestruct (partition_model_disjoint'' first descr with "[$]") as %Hfirst_descr; [done.. |].
-    iSteps as (cl (descr' & -> & Hdescr_elem')%elem_of_map) / --silent. iPureIntro.
+    iDestruct (partition_model_disjoint'' class descr first with "[$]") as %?; [done.. |].
+    iSteps as (cl (class' & descr' & Hdescrs_lookup' & <-)%elem_of_map_to_set) / --silent. iPureIntro.
     rewrite !elem_of_list_to_set. naive_solver.
   Qed.
 
@@ -575,14 +541,14 @@ Section partition_G.
   Proof.
     iIntros "%Φ ((:model) & Helt) HΦ".
     wp_rec.
-    wp_apply (partition_get_class_spec with "[$Hmodel $Helt]") as (descr) "(Hmodel & Helt & %Hdescrs_elem & %Helts_elem & %Helt_descr)".
-    iDestruct (partition_model_descr_elts_NoDup with "Hmodel") as %?; first done.
+    wp_apply (partition_get_class_spec with "[$Hmodel $Helt]") as (class descr) "(Hmodel & Helt & %Hdescrs_lookup & %Helts_elem & %Helt)".
+    iDestruct (partition_descr_model_elts_NoDup with "Hmodel") as %?; first done.
     iDestruct "Hmodel" as "(:model')".
-    iDestruct (big_sepS_elem_of_acc with "Hdescrs") as "((:model_descr) & Hdescrs)"; first done.
+    iDestruct (big_sepM_lookup_acc with "Hdescrs") as "((:descr_model) & Hdescrs)"; first done.
     wp_load.
-    iDestruct ("Hdescrs" with "[- Helts_auth Helt HΦ]") as "Hdescrs".
-    { iExists first, last, prev_descr, prev, next_descr, next. iSteps. }
-    iSteps as (cl (descr' & -> & Hdescr_elem')%elem_of_map ->%elem_of_list_to_set%Helt_descr) / --silent; last done. iPureIntro.
+    iDestruct ("Hdescrs" with "[- Helts_auth Helt HΦ]") as "Hdescrs"; first iSteps.
+    iSteps as (cl (class' & descr' & Hdescrs_lookup' & <-)%elem_of_map_to_set Helts'_elem%elem_of_list_to_set) / --silent. iPureIntro.
+    edestruct (Helt class' descr') as (-> & ->); [done.. |].
     rewrite size_list_to_set //.
   Qed.
 
